c_stubs/tls13_io_stubs.h
@@ -1,0 +1,9 @@
+#ifndef TLS13_IO_STUBS_H
+#define TLS13_IO_STUBS_H
+
+#include <stdbool.h>
+#include <stddef.h>
+#include <stdint.h>
+
+#endif
+
