c_stubs/tls13_wire_stubs.h
@@ -1,0 +1,9 @@
+#ifndef TLS13_WIRE_STUBS_H
+#define TLS13_WIRE_STUBS_H
+
+#include <stdbool.h>
+#include <stddef.h>
+#include <stdint.h>
+
+#endif
+
