src/impl/TLS13.IO.fsti
@@ -1,0 +1,26 @@
+module TLS13.IO
+
+#lang-pulse
+
+open Pulse.Lib.Pervasives
+open Pulse.Lib.Array.PtsTo
+
+module B = TLS13.Bytes
+module SZ = FStar.SizeT
+module U8 = FStar.UInt8
+
+val channel : Type0
+val is_channel: channel -> slprop
+
+fn read (ch: channel) (out: array U8.t) (max_len: SZ.t)
+  requires is_channel ch ** pts_to out 'old ** pure (B.length 'old == SZ.v max_len)
+  returns n: SZ.t
+  ensures exists* bytes. is_channel ch **
+          pts_to out bytes **
+          pure (B.length bytes == SZ.v max_len /\ SZ.v n <= SZ.v max_len)
+
+fn write (ch: channel) (buf: array U8.t) (len: SZ.t)
+  requires is_channel ch ** pts_to buf 'bytes ** pure (B.length 'bytes == SZ.v len)
+  returns n: SZ.t
+  ensures is_channel ch ** pts_to buf 'bytes ** pure (SZ.v n <= SZ.v len)
+
