src/impl/TLS13.LowTypes.fsti
@@ -11,4 +11,3 @@ type u16 = U16.t
 type u32 = U32.t
 type u64 = U64.t
 type size_t = SZ.t
-
