src/impl/TLS13.Parse.fsti
@@ -1,0 +1,21 @@
+module TLS13.Parse
+
+#lang-pulse
+
+open Pulse.Lib.Pervasives
+open Pulse.Lib.Array.PtsTo
+
+module B = TLS13.Bytes
+module SZ = FStar.SizeT
+module U8 = FStar.UInt8
+module W = TLS13.Wire.Spec
+
+fn parse_handshake (input: array U8.t) (input_len: SZ.t)
+  requires pts_to input 'bytes ** pure (B.length 'bytes == SZ.v input_len)
+  returns parsed: option (TLS13.Handshake.Spec.handshake_msg & nat)
+  ensures pts_to input 'bytes ** pure (parsed == W.parse_handshake (Ghost.reveal 'bytes))
+
+fn parse_record (input: array U8.t) (input_len: SZ.t)
+  requires pts_to input 'bytes ** pure (B.length 'bytes == SZ.v input_len)
+  returns parsed: option (TLS13.Types.content_type & TLS13.Record.Spec.sealed_record & nat)
+  ensures pts_to input 'bytes ** pure (parsed == W.parse_record (Ghost.reveal 'bytes))
