src/impl/TLS13.X509.fsti
@@ -1,0 +1,35 @@
+module TLS13.X509
+
+#lang-pulse
+
+open Pulse.Lib.Pervasives
+open Pulse.Lib.Array.PtsTo
+
+module B = TLS13.Bytes
+module SZ = FStar.SizeT
+module U8 = FStar.UInt8
+module X = TLS13.X509.Spec
+
+val validation_context : Type0
+val is_validation_context: validation_context -> X.trust_store -> X.validation_time -> slprop
+
+fn validate_chain
+  (ctx: validation_context)
+  (hostname: array U8.t)
+  (hostname_len: SZ.t)
+  (certs: array U8.t)
+  (certs_len: SZ.t)
+  requires is_validation_context ctx 'trust_store 'validation_time **
+           pts_to hostname 'hostname_bytes **
+           pts_to certs 'cert_bytes **
+           pure (B.length 'hostname_bytes == SZ.v hostname_len /\
+                 B.length 'cert_bytes == SZ.v certs_len)
+  returns peer: option X.peer_identity
+  ensures is_validation_context ctx 'trust_store 'validation_time **
+          pts_to hostname 'hostname_bytes **
+          pts_to certs 'cert_bytes **
+          pure (peer == X.validate_chain
+                          (Ghost.reveal 'hostname_bytes)
+                          'validation_time
+                          'trust_store
+                          [Ghost.reveal 'cert_bytes])
