src/spec/TLS13.Wire.Spec.fsti
@@ -1,0 +1,25 @@
+module TLS13.Wire.Spec
+
+module B = TLS13.Bytes
+module H = TLS13.Handshake.Spec
+module R = TLS13.Record.Spec
+module T = TLS13.Types
+
+type parse_error = T.tls_error
+
+val parse_handshake:
+  input:B.bytes ->
+  Tot (option (H.handshake_msg & nat))
+
+val serialize_handshake:
+  msg:H.handshake_msg ->
+  Tot B.bytes
+
+val parse_record:
+  input:B.bytes ->
+  Tot (option (T.content_type & R.sealed_record & nat))
+
+val serialize_record:
+  content_type:T.content_type ->
+  fragment:B.bytes ->
+  Tot B.bytes
